荷物
```math
q=\begin{pmatrix}
q_{1}\\
q_{2}\\
q_{3}\\
\end{pmatrix}
```

重み係数
```math
A=\begin{pmatrix}
A_{1,1} \ A_{1,2} \\
A_{2,1} \ A_{2,2} \\
A_{3,1} \ A_{3,2} \\
\end{pmatrix}
```

期待値
```math
V=\begin{pmatrix}
q_{1} A_{1,1} \ q_{1}A_{1,2} \\
q_{2} A_{2,1} \ q_{2}A_{2,2} \\
q_{3} A_{3,1} \ q_{3}A_{3,2} \\
\end{pmatrix}=\begin{pmatrix}
V_{1,1} \ V_{1,2} \\
V_{2,1} \ V_{2,2} \\
V_{3,1} \ V_{3,2} \\
\end{pmatrix}
```
固定値
```math
C=\begin{pmatrix}
C_{1}\\
C_{2}\\
\end{pmatrix}
```

求めたい値
```math
X=\begin{pmatrix}
X_{1}\\
X_{2}\\
X_{3}\\
\end{pmatrix}
```

```math
XC^T=
\begin{pmatrix}
X_{1} C_{1} \ X_{1}C_{2} \\
X_{2} C_{1} \ X_{2}C_{2} \\
X_{3} C_{1} \ X_{3}C_{2} \\
\end{pmatrix} \\

P_1 = 
\begin{pmatrix}
(X_{1} C_{1} + X_{1}C_{2}) - (V_{1,1} + V_{1,2}) \\
(X_{2} C_{1} + X_{2}C_{2}) - (V_{2,1} + V_{2,2}) \\
(X_{3} C_{1} + X_{3}C_{2}) - (V_{3,1} + V_{3,2}) \\
\end{pmatrix} \\
=\begin{pmatrix}
(C_{1} + C_{2})X_{1} - (V_{1,1} + V_{1,2}) \\
(C_{1} + C_{2})X_{2} - (V_{2,1} + V_{2,2}) \\
(C_{1} + C_{2})X_{3} - (V_{3,1} + V_{3,2}) \\
\end{pmatrix} \\
=\begin{pmatrix}
C'X_{1} - V'_{1} \\
C'X_{2} - V'_{2} \\
C'X_{3} - V'_{3} \\
\end{pmatrix} \\

P_2 =
\begin{pmatrix}
(X_{1} C_{1} + X_{2}C_{1} + X_{3}C_{1}) - (V_{1,1} + V_{2,1} + V_{3,1}) \\
(X_{1} C_{2} + X_{2}C_{2} + X_{3}C_{2}) - (V_{1,2} + V_{2,2} + V_{3,2}) \\
\end{pmatrix} \\
=\begin{pmatrix}
C_{1}X_{1} + C_{1}X_{2} + C_{1}X_{3} - V''_{1} \\
C_{2}X_{1} + C_{2}X_{2} + C_{2}X_{3} - V''_{2} \\
\end{pmatrix} \\

Cost(X) = \frac{1}{2}P_1^TP_1 + P_2^TP_2=\\
\frac{1}{2} ((C'X_1-V'_1)^2 + (C'X_2-V'_2)^2 + (C'X_3-V'_3)^2 + 
(C_{1}X_{1} + C_{1}X_{2} + C_{1}X_{3} - V''_{1})^2 +
(C_{2}X_{1} + C_{2}X_{2} + C_{2}X_{3} - V''_{2})^2) \\
\frac{\partial}{\partial X_1} Cost(X) =
C'^2X_1 - V'_1 +
C_1^2 X_1 + C_1 (C_{1}X_{2} + C_{1}X_{3} - V''_{1}) +
C_2^2 X_2 + C_2 (C_{2}X_{2} + C_{2}X_{3} - V''_{2}) \\
= (C'^2+C_1^2+C_2^2)X_1 + (C_1^2+C_2^2)X_2 + (C_1^2+C_2^2)X_3 
- (V'_1 + C_1V''_1 + C_2V''_2) \\
= (S + T)X_1 + TX_2 + TX_3 - (V'_1 + U) \\

\frac{\partial}{\partial X_2} Cost(X) = TX_1 + (S + T)X_2 + TX_3 - (V'_2 + U) \\

\frac{\partial}{\partial X_3} Cost(X) = TX_1 + TX_2 + (S + T)X_3 - (V'_3 + U) \\

```

```math

\begin{pmatrix}
(S + T) \ T \ T \\
T \ (S + T) \ T \\
T \ T \ (S + T) \\
\end{pmatrix} 
X
=\begin{pmatrix}
V'_{1} + U \\
V'_{2} + U \\
V'_{3} + U \\
\end{pmatrix} \\

\begin{pmatrix}
(S + T) \ T \ T \\
-S \ S \ 0 \\
-S \ 0 \ S \\
\end{pmatrix} 
X
=\begin{pmatrix}
V'_{1} + U \\
V'_{2} - V'_{1} \\
V'_{3} - V'_{1} \\
\end{pmatrix} \\

\begin{pmatrix}
(S + 3T) \ 0 \ 0 \\
-S \ S \ 0 \\
-S \ 0 \ S \\
\end{pmatrix} 
X
=\begin{pmatrix}
V'_{1} + U - \frac{T}{S}(V'_{2} + V'_{3} - 2V'_{1}) \\
V'_{2} - V'_{1} \\
V'_{3} - V'_{1} \\
\end{pmatrix} \\
=\begin{pmatrix}
U + \frac{S + 2T}{S}V'_{1} - \frac{T}{S}V'_{2} - \frac{T}{S} V'_{3} \\
V'_{2} - V'_{1} \\
V'_{3} - V'_{1} \\
\end{pmatrix} \\

\begin{pmatrix}
1 \ 0 \ 0 \\
-1 \ 1 \ 0 \\
-1 \ 0 \ 1 \\
\end{pmatrix} 
X
=\begin{pmatrix}
\frac{1}{S+3T}(U + \frac{S + 2T}{S}V'_{1} - \frac{T}{S}V'_{2} - \frac{T}{S} V'_{3}) \\
\frac{1}{S}(V'_{2} - V'_{1}) \\
\frac{1}{S}(V'_{3} - V'_{1}) \\
\end{pmatrix} \\


\begin{pmatrix}
1 \ 0 \ 0 \\
0 \ 1 \ 0 \\
0 \ 0 \ 1 \\
\end{pmatrix} 
X
=\begin{pmatrix}
\frac{1}{S+3T}(U + \frac{S + 2T}{S}V'_{1} - \frac{T}{S}V'_{2} - \frac{T}{S} V'_{3}) \\
\frac{1}{S+3T}(U - \frac{T}{S}V'_{1} + \frac{S + 2T}{S}V'_{2} - \frac{T}{S} V'_{3}) \\
\frac{1}{S+3T}(U - \frac{T}{S}V'_{1} - \frac{T}{S}V'_{2} + \frac{S + 2T}{S} V'_{3}) \\
\end{pmatrix} \\

```

```math

X=\frac{1}{S+3T} U + \frac{1}{S+3T}\begin{pmatrix}
\frac{S + 2T}{S} \ - \frac{T}{S} \ - \frac{T}{S} \\
 - \frac{T}{S} \ \frac{S + 2T}{S} \ - \frac{T}{S} \\
 - \frac{T}{S} \ - \frac{T}{S} \ \frac{S + 2T}{S} \\
\end{pmatrix} \begin{pmatrix} 
V'_{1} \\
V'_{2} \\
V'_{3} \\
\end{pmatrix} \\
=
\frac{1}{S+3T} U + \frac{1}{S+3T}(\begin{pmatrix}
S + 3T \ 0 \ 0 \\
 0 \ S + 3T \ 0 \\
 0 \ 0 \ S + 3T \\
\end{pmatrix}
- \frac{T}{S})
\begin{pmatrix} 
V'_{1} \\
V'_{2} \\
V'_{3} \\
\end{pmatrix} \\
=
\frac{1}{S+3T} U + (I
- \frac{T}{S(S+3T)})
\begin{pmatrix} 
V'_{1} \\
V'_{2} \\
V'_{3} \\
\end{pmatrix} \\

S = (C_1 + C_2)^2 \\
T = C_1^2+C_2^2 \\
U = C_1(V_{1,1} + V_{2,1} + V_{3,1}) + C_2(V_{1,2} + V_{2,2} + V_{3,2}) \\
V'_i = V_{i,1} + V_{i,2} \\
```
```python
import numpy as np

c = np.array([5.0, 10.0])
q = np.array([10, 15, 20])
A = np.array([[30, 60], [35, 65], [40, 70]])
dimension = 3
V = A * q.reshape(dimension, 1)
V_prime = V.sum(axis=1)
s = np.square(c.sum())
t = np.square(c).sum()
u = (V * c).sum()
VV = V_prime + u
pp = np.matrix([[s+t, t, t], [t, s+t, t], [t, t, s+t]])
x = pp.I @ VV
x = u / (s + 3 * t) + (np.eye(dimension) - t / (s * (s + 3 * t))) @ V_prime
```